providers/evercrypt/EverCrypt.Arm.fsti
@@ -1,0 +1,12 @@
+module EverCrypt.Arm
+
+open FStar.HyperStack.ST
+
+val has_neon: bool
+
+val check_neon: unit -> Stack bool
+  (requires fun _ ->
+    EverCrypt.TargetConfig.(aarch32 || aarch64))
+  (ensures fun h0 b h1 ->
+    h0 == h1 /\ (
+    b ==> has_neon))
